Sources/Doi_10_1145_3737283/Section33.lean
@@ -1,4 +1,8 @@
 import DeepWiki.Refine.Parametricity.Univalent.Package
+import DeepWiki.Refine.Parametricity.Univalent.Syntax
+import DeepWiki.Refine.Parametricity.Univalent.Realizers
+import DeepWiki.Refine.Parametricity.Univalent.Translation
+import DeepWiki.Refine.Parametricity.Univalent.Typing
 import DeepWiki.Refine.Parametricity.Intrinsic.Abstraction
 import DeepWiki.Refine.Parametricity.Raw.Abstraction
 import DeepWiki.Refine.Parametricity.Univalent.Abstraction
